cequiv/approx.v
@@ -2609,10 +2609,3 @@ Qed.
 *)
 
 (* end hide *)
-
-
-(*
-*** Local Variables:
-*** coq-load-path: ("." "../util/" "../terms/" "../computation/")
-*** End:
-*)
